.

statdb-cli/extract/Bool.hs
@@ -1,0 +1,85 @@
+{-# OPTIONS_GHC -F -pgmF ./fiximports.py #-}
+module Bool where
+
+import qualified Prelude
+import qualified Datatypes
+import qualified Logic
+
+__ :: any
+__ = Prelude.error "Logical or arity value used"
+
+bool_dec :: Prelude.Bool -> Prelude.Bool -> Prelude.Bool
+bool_dec b1 b2 =
+  Datatypes.bool_rec (\x ->
+    case x of {
+     Prelude.True -> Prelude.True;
+     Prelude.False -> Prelude.False}) (\x ->
+    case x of {
+     Prelude.True -> Prelude.False;
+     Prelude.False -> Prelude.True}) b1 b2
+
+eqb :: Prelude.Bool -> Prelude.Bool -> Prelude.Bool
+eqb b1 b2 =
+  case b1 of {
+   Prelude.True -> b2;
+   Prelude.False ->
+    case b2 of {
+     Prelude.True -> Prelude.False;
+     Prelude.False -> Prelude.True}}
+
+ifb :: Prelude.Bool -> Prelude.Bool -> Prelude.Bool -> Prelude.Bool
+ifb b1 b2 b3 =
+  case b1 of {
+   Prelude.True -> b2;
+   Prelude.False -> b3}
+
+orb_true_elim :: Prelude.Bool -> Prelude.Bool -> Prelude.Bool
+orb_true_elim b1 _ =
+  case b1 of {
+   Prelude.True -> Prelude.True;
+   Prelude.False -> Prelude.False}
+
+andb_false_elim :: Prelude.Bool -> Prelude.Bool -> Prelude.Bool
+andb_false_elim b1 _ =
+  case b1 of {
+   Prelude.True -> Prelude.False;
+   Prelude.False -> Prelude.True}
+
+data Coq_reflect =
+   ReflectT
+ | ReflectF
+
+reflect_rect :: (() -> a1) -> (() -> a1) -> Prelude.Bool -> Coq_reflect -> a1
+reflect_rect f f0 _ r =
+  case r of {
+   ReflectT -> f __;
+   ReflectF -> f0 __}
+
+reflect_rec :: (() -> a1) -> (() -> a1) -> Prelude.Bool -> Coq_reflect -> a1
+reflect_rec =
+  reflect_rect
+
+iff_reflect :: Prelude.Bool -> Coq_reflect
+iff_reflect b =
+  case b of {
+   Prelude.True -> Logic.and_rec (\_ _ -> ReflectT);
+   Prelude.False -> Logic.and_rec (\_ _ -> ReflectF)}
+
+reflect_dec :: Prelude.Bool -> Coq_reflect -> Prelude.Bool
+reflect_dec _ h =
+  case h of {
+   ReflectT -> Prelude.True;
+   ReflectF -> Prelude.False}
+
+eqb_spec :: Prelude.Bool -> Prelude.Bool -> Coq_reflect
+eqb_spec b b' =
+  case b of {
+   Prelude.True ->
+    case b' of {
+     Prelude.True -> ReflectT;
+     Prelude.False -> ReflectF};
+   Prelude.False ->
+    case b' of {
+     Prelude.True -> ReflectF;
+     Prelude.False -> ReflectT}}
+
