statdb-cli/extract/Datatypes.hs
@@ -1,0 +1,239 @@
+{-# OPTIONS_GHC -F -pgmF ./fiximports.py #-}
+{-# OPTIONS_GHC -cpp -XMagicHash #-}
+{- For Hugs, use the option -F"cpp -P -traditional" -}
+
+module Datatypes where
+
+import qualified Prelude
+
+#ifdef __GLASGOW_HASKELL__
+import qualified GHC.Base
+#else
+-- HUGS
+import qualified IOExts
+#endif
+
+#ifdef __GLASGOW_HASKELL__
+type Any = GHC.Base.Any
+#else
+-- HUGS
+type Any = ()
+#endif
+
+__ :: any
+__ = Prelude.error "Logical or arity value used"
+
+type Empty_set = () -- empty inductive
+
+coq_Empty_set_rect :: Empty_set -> a1
+coq_Empty_set_rect _ =
+  Prelude.error "absurd case"
+
+coq_Empty_set_rec :: Empty_set -> a1
+coq_Empty_set_rec =
+  coq_Empty_set_rect
+
+unit_rect :: a1 -> () -> a1
+unit_rect f _ =
+  f
+
+unit_rec :: a1 -> () -> a1
+unit_rec =
+  unit_rect
+
+bool_rect :: a1 -> a1 -> Prelude.Bool -> a1
+bool_rect f f0 b =
+  case b of {
+   Prelude.True -> f;
+   Prelude.False -> f0}
+
+bool_rec :: a1 -> a1 -> Prelude.Bool -> a1
+bool_rec =
+  bool_rect
+
+implb :: Prelude.Bool -> Prelude.Bool -> Prelude.Bool
+implb b1 b2 =
+  case b1 of {
+   Prelude.True -> b2;
+   Prelude.False -> Prelude.True}
+
+xorb :: Prelude.Bool -> Prelude.Bool -> Prelude.Bool
+xorb b1 b2 =
+  case b1 of {
+   Prelude.True ->
+    case b2 of {
+     Prelude.True -> Prelude.False;
+     Prelude.False -> Prelude.True};
+   Prelude.False -> b2}
+
+eq_true_rect :: a1 -> Prelude.Bool -> a1
+eq_true_rect f _ =
+  f
+
+eq_true_rec :: a1 -> Prelude.Bool -> a1
+eq_true_rec =
+  eq_true_rect
+
+eq_true_rec_r :: Prelude.Bool -> a1 -> a1
+eq_true_rec_r _ h =
+  h
+
+eq_true_rect_r :: Prelude.Bool -> a1 -> a1
+eq_true_rect_r _ h =
+  h
+
+nat_rect :: a1 -> (Prelude.Integer -> a1 -> a1) -> Prelude.Integer -> a1
+nat_rect f f0 n =
+  (\fO fS n -> if n Prelude.== 0 then fO () else fS (n Prelude.- 1))
+    (\_ -> f)
+    (\n0 -> f0 n0 (nat_rect f f0 n0))
+    n
+
+nat_rec :: a1 -> (Prelude.Integer -> a1 -> a1) -> Prelude.Integer -> a1
+nat_rec =
+  nat_rect
+
+option_rect :: (a1 -> a2) -> a2 -> (Prelude.Maybe a1) -> a2
+option_rect f f0 o =
+  case o of {
+   Prelude.Just x -> f x;
+   Prelude.Nothing -> f0}
+
+option_rec :: (a1 -> a2) -> a2 -> (Prelude.Maybe a1) -> a2
+option_rec =
+  option_rect
+
+option_map :: (a1 -> a2) -> (Prelude.Maybe a1) -> Prelude.Maybe a2
+option_map f o =
+  case o of {
+   Prelude.Just a -> Prelude.Just (f a);
+   Prelude.Nothing -> Prelude.Nothing}
+
+sum_rect :: (a1 -> a3) -> (a2 -> a3) -> (Prelude.Either a1 a2) -> a3
+sum_rect f f0 s =
+  case s of {
+   Prelude.Left x -> f x;
+   Prelude.Right x -> f0 x}
+
+sum_rec :: (a1 -> a3) -> (a2 -> a3) -> (Prelude.Either a1 a2) -> a3
+sum_rec =
+  sum_rect
+
+prod_rect :: (a1 -> a2 -> a3) -> ((,) a1 a2) -> a3
+prod_rect f p =
+  case p of {
+   (,) x x0 -> f x x0}
+
+prod_rec :: (a1 -> a2 -> a3) -> ((,) a1 a2) -> a3
+prod_rec =
+  prod_rect
+
+fst :: ((,) a1 a2) -> a1
+fst p =
+  case p of {
+   (,) x _ -> x}
+
+snd :: ((,) a1 a2) -> a2
+snd p =
+  case p of {
+   (,) _ y -> y}
+
+prod_uncurry :: (((,) a1 a2) -> a3) -> a1 -> a2 -> a3
+prod_uncurry f x y =
+  f ((,) x y)
+
+prod_curry :: (a1 -> a2 -> a3) -> ((,) a1 a2) -> a3
+prod_curry f p =
+  case p of {
+   (,) x y -> f x y}
+
+list_rect :: a2 -> (a1 -> (([]) a1) -> a2 -> a2) -> (([]) a1) -> a2
+list_rect f f0 l =
+  case l of {
+   ([]) -> f;
+   (:) y l0 -> f0 y l0 (list_rect f f0 l0)}
+
+list_rec :: a2 -> (a1 -> (([]) a1) -> a2 -> a2) -> (([]) a1) -> a2
+list_rec =
+  list_rect
+
+length :: (([]) a1) -> Prelude.Integer
+length l =
+  case l of {
+   ([]) -> 0;
+   (:) _ l' -> Prelude.succ (length l')}
+
+app :: (([]) a1) -> (([]) a1) -> ([]) a1
+app l m =
+  case l of {
+   ([]) -> m;
+   (:) a l1 -> (:) a (app l1 m)}
+
+data Coq_comparison =
+   Eq
+ | Lt
+ | Gt
+
+comparison_rect :: a1 -> a1 -> a1 -> Coq_comparison -> a1
+comparison_rect f f0 f1 c =
+  case c of {
+   Eq -> f;
+   Lt -> f0;
+   Gt -> f1}
+
+comparison_rec :: a1 -> a1 -> a1 -> Coq_comparison -> a1
+comparison_rec =
+  comparison_rect
+
+coq_CompOpp :: Coq_comparison -> Coq_comparison
+coq_CompOpp r =
+  case r of {
+   Eq -> Eq;
+   Lt -> Gt;
+   Gt -> Lt}
+
+data CompareSpecT =
+   CompEqT
+ | CompLtT
+ | CompGtT
+
+coq_CompareSpecT_rect :: (() -> a1) -> (() -> a1) -> (() -> a1) ->
+                         Coq_comparison -> CompareSpecT -> a1
+coq_CompareSpecT_rect f f0 f1 _ c =
+  case c of {
+   CompEqT -> f __;
+   CompLtT -> f0 __;
+   CompGtT -> f1 __}
+
+coq_CompareSpecT_rec :: (() -> a1) -> (() -> a1) -> (() -> a1) ->
+                        Coq_comparison -> CompareSpecT -> a1
+coq_CompareSpecT_rec =
+  coq_CompareSpecT_rect
+
+coq_CompareSpec2Type :: Coq_comparison -> CompareSpecT
+coq_CompareSpec2Type c =
+  case c of {
+   Eq -> CompEqT;
+   Lt -> CompLtT;
+   Gt -> CompGtT}
+
+type CompSpecT a = CompareSpecT
+
+coq_CompSpec2Type :: a1 -> a1 -> Coq_comparison -> CompSpecT a1
+coq_CompSpec2Type _ _ =
+  coq_CompareSpec2Type
+
+identity_rect :: a1 -> a2 -> a1 -> a2
+identity_rect _ f _ =
+  f
+
+identity_rec :: a1 -> a2 -> a1 -> a2
+identity_rec =
+  identity_rect
+
+type ID = () -> Any -> Any
+
+id :: a1 -> a1
+id x =
+  x
+
