statdb-cli/extract/Decimal.hs
@@ -1,0 +1,157 @@
+{-# OPTIONS_GHC -F -pgmF ./fiximports.py #-}
+module Decimal where
+
+import qualified Prelude
+
+data Coq_uint =
+   Nil
+ | D0 Coq_uint
+ | D1 Coq_uint
+ | D2 Coq_uint
+ | D3 Coq_uint
+ | D4 Coq_uint
+ | D5 Coq_uint
+ | D6 Coq_uint
+ | D7 Coq_uint
+ | D8 Coq_uint
+ | D9 Coq_uint
+
+uint_rect :: a1 -> (Coq_uint -> a1 -> a1) -> (Coq_uint -> a1 -> a1) ->
+             (Coq_uint -> a1 -> a1) -> (Coq_uint -> a1 -> a1) -> (Coq_uint ->
+             a1 -> a1) -> (Coq_uint -> a1 -> a1) -> (Coq_uint -> a1 -> a1) ->
+             (Coq_uint -> a1 -> a1) -> (Coq_uint -> a1 -> a1) -> (Coq_uint ->
+             a1 -> a1) -> Coq_uint -> a1
+uint_rect f f0 f1 f2 f3 f4 f5 f6 f7 f8 f9 u =
+  case u of {
+   Nil -> f;
+   D0 u0 -> f0 u0 (uint_rect f f0 f1 f2 f3 f4 f5 f6 f7 f8 f9 u0);
+   D1 u0 -> f1 u0 (uint_rect f f0 f1 f2 f3 f4 f5 f6 f7 f8 f9 u0);
+   D2 u0 -> f2 u0 (uint_rect f f0 f1 f2 f3 f4 f5 f6 f7 f8 f9 u0);
+   D3 u0 -> f3 u0 (uint_rect f f0 f1 f2 f3 f4 f5 f6 f7 f8 f9 u0);
+   D4 u0 -> f4 u0 (uint_rect f f0 f1 f2 f3 f4 f5 f6 f7 f8 f9 u0);
+   D5 u0 -> f5 u0 (uint_rect f f0 f1 f2 f3 f4 f5 f6 f7 f8 f9 u0);
+   D6 u0 -> f6 u0 (uint_rect f f0 f1 f2 f3 f4 f5 f6 f7 f8 f9 u0);
+   D7 u0 -> f7 u0 (uint_rect f f0 f1 f2 f3 f4 f5 f6 f7 f8 f9 u0);
+   D8 u0 -> f8 u0 (uint_rect f f0 f1 f2 f3 f4 f5 f6 f7 f8 f9 u0);
+   D9 u0 -> f9 u0 (uint_rect f f0 f1 f2 f3 f4 f5 f6 f7 f8 f9 u0)}
+
+uint_rec :: a1 -> (Coq_uint -> a1 -> a1) -> (Coq_uint -> a1 -> a1) ->
+            (Coq_uint -> a1 -> a1) -> (Coq_uint -> a1 -> a1) -> (Coq_uint ->
+            a1 -> a1) -> (Coq_uint -> a1 -> a1) -> (Coq_uint -> a1 -> a1) ->
+            (Coq_uint -> a1 -> a1) -> (Coq_uint -> a1 -> a1) -> (Coq_uint ->
+            a1 -> a1) -> Coq_uint -> a1
+uint_rec =
+  uint_rect
+
+data Coq_int =
+   Pos Coq_uint
+ | Neg Coq_uint
+
+int_rect :: (Coq_uint -> a1) -> (Coq_uint -> a1) -> Coq_int -> a1
+int_rect f f0 i =
+  case i of {
+   Pos x -> f x;
+   Neg x -> f0 x}
+
+int_rec :: (Coq_uint -> a1) -> (Coq_uint -> a1) -> Coq_int -> a1
+int_rec =
+  int_rect
+
+nzhead :: Coq_uint -> Coq_uint
+nzhead d =
+  case d of {
+   D0 d0 -> nzhead d0;
+   _ -> d}
+
+unorm :: Coq_uint -> Coq_uint
+unorm d =
+  case nzhead d of {
+   Nil -> D0 Nil;
+   x -> x}
+
+norm :: Coq_int -> Coq_int
+norm d =
+  case d of {
+   Pos d0 -> Pos (unorm d0);
+   Neg d0 -> case nzhead d0 of {
+              Nil -> Pos (D0 Nil);
+              x -> Neg x}}
+
+opp :: Coq_int -> Coq_int
+opp d =
+  case d of {
+   Pos d0 -> Neg d0;
+   Neg d0 -> Pos d0}
+
+revapp :: Coq_uint -> Coq_uint -> Coq_uint
+revapp d d' =
+  case d of {
+   Nil -> d';
+   D0 d0 -> revapp d0 (D0 d');
+   D1 d0 -> revapp d0 (D1 d');
+   D2 d0 -> revapp d0 (D2 d');
+   D3 d0 -> revapp d0 (D3 d');
+   D4 d0 -> revapp d0 (D4 d');
+   D5 d0 -> revapp d0 (D5 d');
+   D6 d0 -> revapp d0 (D6 d');
+   D7 d0 -> revapp d0 (D7 d');
+   D8 d0 -> revapp d0 (D8 d');
+   D9 d0 -> revapp d0 (D9 d')}
+
+rev :: Coq_uint -> Coq_uint
+rev d =
+  revapp d Nil
+
+_Little__succ :: Coq_uint -> Coq_uint
+_Little__succ d =
+  case d of {
+   Nil -> D1 Nil;
+   D0 d0 -> D1 d0;
+   D1 d0 -> D2 d0;
+   D2 d0 -> D3 d0;
+   D3 d0 -> D4 d0;
+   D4 d0 -> D5 d0;
+   D5 d0 -> D6 d0;
+   D6 d0 -> D7 d0;
+   D7 d0 -> D8 d0;
+   D8 d0 -> D9 d0;
+   D9 d0 -> D0 (_Little__succ d0)}
+
+_Little__double :: Coq_uint -> Coq_uint
+_Little__double d =
+  case d of {
+   Nil -> Nil;
+   D0 d0 -> D0 (_Little__double d0);
+   D1 d0 -> D2 (_Little__double d0);
+   D2 d0 -> D4 (_Little__double d0);
+   D3 d0 -> D6 (_Little__double d0);
+   D4 d0 -> D8 (_Little__double d0);
+   D5 d0 -> D0 (_Little__succ_double d0);
+   D6 d0 -> D2 (_Little__succ_double d0);
+   D7 d0 -> D4 (_Little__succ_double d0);
+   D8 d0 -> D6 (_Little__succ_double d0);
+   D9 d0 -> D8 (_Little__succ_double d0)}
+
+_Little__succ_double :: Coq_uint -> Coq_uint
+_Little__succ_double d =
+  case d of {
+   Nil -> D1 Nil;
+   D0 d0 -> D1 (_Little__double d0);
+   D1 d0 -> D3 (_Little__double d0);
+   D2 d0 -> D5 (_Little__double d0);
+   D3 d0 -> D7 (_Little__double d0);
+   D4 d0 -> D9 (_Little__double d0);
+   D5 d0 -> D1 (_Little__succ_double d0);
+   D6 d0 -> D3 (_Little__succ_double d0);
+   D7 d0 -> D5 (_Little__succ_double d0);
+   D8 d0 -> D7 (_Little__succ_double d0);
+   D9 d0 -> D9 (_Little__succ_double d0)}
+
+uint_of_uint :: Coq_uint -> Coq_uint
+uint_of_uint i =
+  i
+
+int_of_int :: Coq_int -> Coq_int
+int_of_int i =
+  i
+
