statdb-cli/extract/Helpers.hs
@@ -1,0 +1,20 @@
+{-# OPTIONS_GHC -F -pgmF ./fiximports.py #-}
+module Helpers where
+
+import qualified Prelude
+import qualified Bool
+
+type EqualDec a = a -> a -> Prelude.Bool
+
+equal_dec :: (EqualDec a1) -> a1 -> a1 -> Prelude.Bool
+equal_dec equalDec =
+  equalDec
+
+nat_equal_dec :: EqualDec Prelude.Integer
+nat_equal_dec =
+  (Prelude.==)
+
+bool_equal_dec :: EqualDec Prelude.Bool
+bool_equal_dec =
+  Bool.bool_dec
+
