statdb-cli/extract/Nat.hs
@@ -1,0 +1,5 @@
+{-# OPTIONS_GHC -F -pgmF ./fiximports.py #-}
+module Nat where
+
+import qualified Prelude
+
