statdb-cli/extract/Proc.hs
@@ -1,0 +1,30 @@
+{-# OPTIONS_GHC -F -pgmF ./fiximports.py #-}
+{-# OPTIONS_GHC -cpp -XMagicHash #-}
+{- For Hugs, use the option -F"cpp -P -traditional" -}
+
+module Proc where
+
+import qualified Prelude
+
+#ifdef __GLASGOW_HASKELL__
+import qualified GHC.Base
+#else
+-- HUGS
+import qualified IOExts
+#endif
+
+#ifdef __GLASGOW_HASKELL__
+type Any = GHC.Base.Any
+#else
+-- HUGS
+type Any = ()
+#endif
+
+type IO__Coq_baseOpT x = Any
+
+type IO__Coq_world = Any
+
+type Coq_baseOpT x = IO__Coq_baseOpT x
+
+type Coq_world = IO__Coq_world
+
