statdb-cli/extract/StatDbCli.hs
@@ -1,0 +1,90 @@
+{-# OPTIONS_GHC -F -pgmF ./fiximports.py #-}
+{-# OPTIONS_GHC -cpp -XMagicHash #-}
+{- For Hugs, use the option -F"cpp -P -traditional" -}
+
+module StatDbCli where
+
+import qualified Prelude
+import qualified Abstraction
+import qualified StatDbAPI
+import qualified VariablesAPI
+import qualified VariablesImpl
+
+#ifdef __GLASGOW_HASKELL__
+import qualified GHC.Base
+#else
+-- HUGS
+import qualified IOExts
+#endif
+
+#ifdef __GLASGOW_HASKELL__
+unsafeCoerce :: a -> b
+unsafeCoerce = GHC.Base.unsafeCoerce#
+#else
+-- HUGS
+unsafeCoerce :: a -> b
+unsafeCoerce = IOExts.unsafeCoerce
+#endif
+
+_Coq_statdb__add :: Prelude.Integer -> Proc ()
+_Coq_statdb__add v =
+  (>>=) (unsafeCoerce VariablesImpl._Vars__read VariablesAPI.VarSum) (\sum ->
+    (>>=) (unsafeCoerce VariablesImpl._Vars__read VariablesAPI.VarCount)
+    (\count -> (>>=)
+    (unsafeCoerce VariablesImpl._Vars__write VariablesAPI.VarSum
+      ((Prelude.+) (unsafeCoerce sum) v)) (\_ -> (>>=)
+    (unsafeCoerce VariablesImpl._Vars__write VariablesAPI.VarCount
+      ((Prelude.+) (unsafeCoerce count) (Prelude.succ 0))) (\_ -> return
+    ()))))
+
+_Coq_statdb__mean :: Proc (Prelude.Maybe Prelude.Integer)
+_Coq_statdb__mean =
+  (>>=) (unsafeCoerce VariablesImpl._Vars__read VariablesAPI.VarSum) (\sum ->
+    (>>=) (unsafeCoerce VariablesImpl._Vars__read VariablesAPI.VarCount)
+    (\count ->
+    (\fO fS n -> if n Prelude.== 0 then fO () else fS (n Prelude.- 1))
+      (\_ -> return Prelude.Nothing)
+      (\n -> return (Prelude.Just
+      ((\n m -> if m Prelude.== 0 then 0 else Prelude.div n m)
+        (unsafeCoerce sum) (Prelude.succ n))))
+      (unsafeCoerce count)))
+
+_Coq_statdb__init' :: Proc Abstraction.InitResult
+_Coq_statdb__init' =
+  (>>=) (unsafeCoerce VariablesImpl._Vars__write VariablesAPI.VarCount 0)
+    (\_ -> (>>=)
+    (unsafeCoerce VariablesImpl._Vars__write VariablesAPI.VarSum 0) (\_ ->
+    return Abstraction.Initialized))
+
+_Coq_statdb__init :: Proc Abstraction.InitResult
+_Coq_statdb__init =
+  Abstraction.then_init VariablesImpl._Vars__init _Coq_statdb__init'
+
+_Coq_statdb__recover :: Proc ()
+_Coq_statdb__recover =
+  VariablesImpl._Vars__recover
+
+_Coq_statdb__abstr :: Abstraction.Abstraction StatDbAPI.State
+_Coq_statdb__abstr =
+  Abstraction.abstraction_compose VariablesImpl._Vars__abstr
+    Abstraction.Build_LayerAbstraction
+
+get_new_item :: Proc Prelude.Integer
+get_new_item = CLI.Stubs.getNewItem
+
+report_mean :: (Prelude.Maybe Prelude.Integer) -> Proc ()
+report_mean = CLI.Stubs.reportMean
+
+loop :: Proc ()
+loop =
+  (>>=) (unsafeCoerce _Coq_statdb__mean) (\m -> (>>=)
+    (unsafeCoerce report_mean m) (\_ -> (>>=) (unsafeCoerce get_new_item)
+    (\x -> (>>=) (unsafeCoerce _Coq_statdb__add x) (\_ -> loop))))
+
+cli :: Proc ()
+cli =
+  (>>=) (unsafeCoerce _Coq_statdb__init) (\init_ok ->
+    case unsafeCoerce init_ok of {
+     Abstraction.Initialized -> loop;
+     Abstraction.InitFailed -> return ()})
+
