statdb-cli/extract/VariablesImpl.hs
@@ -1,0 +1,24 @@
+{-# OPTIONS_GHC -F -pgmF ./fiximports.py #-}
+module VariablesImpl where
+
+import qualified Prelude
+import qualified Abstraction
+import qualified VariablesAPI
+
+_Vars__init :: Proc Abstraction.InitResult
+_Vars__init = Variables.Ops.init
+
+_Vars__read :: VariablesAPI.Coq_var -> Proc Prelude.Integer
+_Vars__read = Variables.Ops.read
+
+_Vars__write :: VariablesAPI.Coq_var -> Prelude.Integer -> Proc ()
+_Vars__write = Variables.Ops.write
+
+_Vars__recover :: Proc ()
+_Vars__recover =
+  Prelude.error "AXIOM TO BE REALIZED"
+
+_Vars__abstr :: Abstraction.Abstraction VariablesAPI.State
+_Vars__abstr =
+  Prelude.error "AXIOM TO BE REALIZED"
+
